Proof various lemmas the for new transition tags
  * Proof the integrity of the list of asyncronous transition
    wrt the main transition such that some information can be
    inferred from having a transition

semantics/semBakeryScript.sml
@@ -123,8 +123,97 @@ val (trans_rules,trans_ind,trans_cases) = Hol_reln `
 
 val _ = zip ["trans_com","trans_sel","trans_let","trans_if_true","trans_if_false",
               "trans_if_swap","trans_com_swap","trans_sel_swap","trans_let_swap",
-              "trans_com_asynch","trans_sel_async"]
+              "trans_com_async","trans_sel_async"]
             (CONJUNCTS trans_rules) |> map save_thm;
+
+val trans_pairind = save_thm("trans_pairind",
+  theorem"trans_strongind"
+  |> Q.SPEC `λa0 a1 a2. P (FST a0) (SND a0) (FST a1) (SND a1)  (FST a2) (SND a2)`
+  |> SIMP_RULE std_ss [FORALL_PROD]
+  |> Q.GEN `P`
+);
+
+(* valid_action ensures a transition tag `alpha` and an asyncronous
+   transition tag `h` are related as described in the asyncronous
+   transitions rules (trans_com_async and trans_sel_async).
+
+   For this relation to hold `h` must:
+
+   * Be one of LSel or LCom
+
+   * Have its sender be a free process in `alpha`
+
+   * Don't have as a receiver a free process in `alpha`
+*)
+val valid_action_def = Define`
+  valid_action alpha h = ((∃p1 b p2 .
+                           h = LSel p1 b p2
+                           ∧ p1 ∈ freeprocs alpha
+                           ∧ p2 ∉ freeprocs alpha) ∨
+                          (∃p1 v1 p2 v2.
+                            h = LCom p1 v1 p2 v2
+                            ∧ p1 ∈ freeprocs alpha
+                            ∧ p2 ∉ freeprocs alpha))
+`;
+
+(* Any valid transition ensures the relationship between the
+   transition tag `t` and the head of the asyncronous transitions list
+   `h` is a valid_action
+*)
+val trans_valid_action = Q.store_thm("trans_valid_action",
+  `∀s c s' c' t h l.
+    trans (s,c) (t,h::l) (s',c')
+    ⇒ valid_action t h`,
+  rpt GEN_TAC
+  \\ `∀s c t l' s' c'.
+        trans (s,c) (t,l') (s',c')
+        ⇒ l' = h::l
+        ⇒ valid_action t h`
+     suffices_by (metis_tac [])
+  \\ ho_match_mp_tac trans_pairind
+  \\ rw [trans_rules,valid_action_def]
+  \\ rfs [freeprocs_def, sender_def, receiver_def]
+);
+
+(* Any valid trasition with a non-empty list of asyncronous trasitions
+   implies there exist a transition with the same transition tag
+   and the tail of the asyncronous transition list
+*)
+val trans_async_some_trans = Q.store_thm("trans_async_some_trans",
+  `∀s c s' c' t h l.
+    trans (s,c) (t,h::l) (s',c')
+    ⇒ ∃s1 c1 s1' c1'. trans (s1,c1) (t,l) (s1',c1')`,
+  rpt GEN_TAC
+  \\ `∀s c t l' s' c'.
+        trans (s,c) (t,l') (s',c')
+        ⇒ l' = h::l
+        ⇒ ∃s1 c1 s1' c1'. trans (s1,c1) (t,l) (s1',c1')`
+     suffices_by (metis_tac [])
+  \\ ho_match_mp_tac trans_pairind
+  \\ rw [trans_rules]
+  \\ metis_tac []
+);
+
+(* valid_actions over a list of actions *)
+val valid_actions_def   = Define`
+  valid_actions alpha l = EVERY (valid_action alpha) l
+`;
+
+
+(* Any valid transition ensures that both transition tag `t` and
+   asyncronous transitions list `l` satisfies valid_actions
+*)
+val trans_valid_actions = Q.store_thm("trans_valid_actions",
+  `∀s c s' c' t l.
+    trans (s,c) (t,l) (s',c')
+    ⇒ valid_actions t l`,
+  Induct_on `l` >> rw []
+  >- rw [valid_actions_def]
+  \\ IMP_RES_TAC trans_valid_action
+  \\ IMP_RES_TAC trans_async_some_trans
+  \\ `valid_actions t l` by metis_tac []
+  \\ fs [valid_actions_def]
+);
 
 (* Reflexive transitive closure *)
 val trans_s_def = Define`
